code/rsapss/Hacl.RSAPSS.fst
@@ -15,39 +15,42 @@ module BD = Hacl.Bignum.Definitions
 
 #reset-options "--z3rlimit 50 --fuel 0 --ifuel 0"
 
-val rsapss_sign: len:BN.meta_len U64 -> RI.rsapss_sign_st U64 (BE.mk_runtime_exp_uint64 len).BE.mont.BM.bn.BN.len
+inline_for_extraction noextract
+let t_limbs = U64
+
+val rsapss_sign: len:BN.meta_len t_limbs -> RI.rsapss_sign_st t_limbs (BE.mk_runtime_exp len).BE.mont.BM.bn.BN.len
 let rsapss_sign len a modBits eBits dBits skey sLen salt msgLen msg sgnt =
-  RI.rsapss_sign (BE.mk_runtime_exp_uint64 len) a modBits eBits dBits skey sLen salt msgLen msg sgnt
+  RI.rsapss_sign (BE.mk_runtime_exp len) a modBits eBits dBits skey sLen salt msgLen msg sgnt
 
 
-val rsapss_verify: len:BN.meta_len U64 -> RI.rsapss_verify_st U64 (BE.mk_runtime_exp_uint64 len).BE.mont.BM.bn.BN.len
+val rsapss_verify: len:BN.meta_len t_limbs -> RI.rsapss_verify_st t_limbs (BE.mk_runtime_exp len).BE.mont.BM.bn.BN.len
 let rsapss_verify len a modBits eBits pkey sLen k sgnt msgLen msg =
-  RI.rsapss_verify (BE.mk_runtime_exp_uint64 len) a modBits eBits pkey sLen k sgnt msgLen msg
+  RI.rsapss_verify (BE.mk_runtime_exp len) a modBits eBits pkey sLen k sgnt msgLen msg
 
 
-val new_rsapss_load_pkey: RK.new_rsapss_load_pkey_st U64
+val new_rsapss_load_pkey: RK.new_rsapss_load_pkey_st t_limbs
 let new_rsapss_load_pkey r modBits eBits nb eb =
-  RK.new_rsapss_load_pkey RK.load_pkey_u64 r modBits eBits nb eb
+  RK.new_rsapss_load_pkey RK.mk_runtime_rsapss_load_keys r modBits eBits nb eb
 
 
-val new_rsapss_load_skey: RK.new_rsapss_load_skey_st U64
+val new_rsapss_load_skey: RK.new_rsapss_load_skey_st t_limbs
 let new_rsapss_load_skey r modBits eBits dBits nb eb db =
-  RK.new_rsapss_load_skey RK.mk_runtime_rsapss_load_keys_uint64 r modBits eBits dBits nb eb db
+  RK.new_rsapss_load_skey RK.mk_runtime_rsapss_load_keys r modBits eBits dBits nb eb db
 
 
-val rsapss_skey_sign: len:BN.meta_len U64 -> RI.rsapss_skey_sign_st U64 (BE.mk_runtime_exp_uint64 len).BE.mont.BM.bn.BN.len
+val rsapss_skey_sign: len:BN.meta_len t_limbs -> RI.rsapss_skey_sign_st t_limbs (BE.mk_runtime_exp len).BE.mont.BM.bn.BN.len
 let rsapss_skey_sign len a modBits eBits dBits nb eb db sLen salt msgLen msg sgnt =
   RI.rsapss_skey_sign
-    (BE.mk_runtime_exp_uint64 len)
-     RK.mk_runtime_rsapss_load_keys_uint64
-    (RI.mk_runtime_rsapss_uint64 len)
+    (BE.mk_runtime_exp len)
+     RK.mk_runtime_rsapss_load_keys
+    (RI.mk_runtime_rsapss len)
     a modBits eBits dBits nb eb db sLen salt msgLen msg sgnt
 
 
-val rsapss_pkey_verify: len:BN.meta_len U64 -> RI.rsapss_pkey_verify_st U64 (BE.mk_runtime_exp_uint64 len).BE.mont.BM.bn.BN.len
+val rsapss_pkey_verify: len:BN.meta_len t_limbs -> RI.rsapss_pkey_verify_st t_limbs (BE.mk_runtime_exp len).BE.mont.BM.bn.BN.len
 let rsapss_pkey_verify len a modBits eBits nb eb sLen k sgnt msgLen msg =
   RI.rsapss_pkey_verify
-    (BE.mk_runtime_exp_uint64 len)
-     RK.mk_runtime_rsapss_load_keys_uint64
-    (RI.mk_runtime_rsapss_uint64 len)
+    (BE.mk_runtime_exp len)
+     RK.mk_runtime_rsapss_load_keys
+    (RI.mk_runtime_rsapss len)
      a modBits eBits nb eb sLen k sgnt msgLen msg
